prooftests/ExampleFromKamiTutorial_proofs.v
@@ -7,9 +7,56 @@ Require Import FunctionalExtensionality.
 
 Set Implicit Arguments.
 
-Theorem producer_consumer_refinement2 (prefix: string):
+Theorem produce_consume_refinement (prefix: string):
+  TraceInclusion (Foo'mod (mkProduceConsume prefix (mkExtCall (prefix--"ext"))))
+                 (flattened_ModWf (module'mkProducerConsumer.wellformed_mkProducerConsumer prefix (mkExtCall (prefix--"ext")))).
+Proof.
+  repeat autounfold with ModuleDefs.
+    unfold TraceInclusion.
+  intros.
+  exists o1, ls1.
+  repeat split; auto; intros; unfold nthProp2; intros; try destruct (nth_error ls1 i) ; auto; repeat split; intros; try firstorder.
+Qed.
+
+Theorem consumer_refinement (prefix: string):
   TraceInclusion (Consumer'mod (mkConsumer prefix (mkExtCall (prefix--"ext")))) (flattened_ModWf (module'mkConsumer.wellformed_mkConsumer prefix (mkExtCall (prefix--"ext")))).
 Proof.
   repeat autounfold with ModuleDefs.
-  apply TraceInclusion_flatten_r.
+    unfold TraceInclusion.
+  intros.
+  exists o1, ls1.
+  repeat split; auto; intros; unfold nthProp2; intros; try destruct (nth_error ls1 i) ; auto; repeat split; intros; try firstorder.
+Qed.
+
+Theorem flattened_producer_consumer_refinement1 (prefix: string):
+  TraceInclusion (Producer'mod (mkProducer prefix (mkConsumer (prefix--"c0") (mkExtCall (prefix--"ext")))))
+		 (flattened_ModWf (module'mkProducer.wellformed_mkProducer prefix(mkConsumer (prefix--"c0") (mkExtCall (prefix--"ext"))))).
+Proof.
+  repeat autounfold with ModuleDefs.
+    unfold TraceInclusion.
+  intros.
+  exists o1, ls1.
+  repeat split; auto; intros; unfold nthProp2; intros; try destruct (nth_error ls1 i) ; auto; repeat split; intros; try firstorder.
+Qed.
+
+Theorem producer_consumer_refinement (prefix: string):
+  TraceInclusion (Producer'mod (mkProducerConsumer prefix (mkExtCall (prefix--"ext"))))
+                 (flattened_ModWf (module'mkProducerConsumer.wellformed_mkProducerConsumer prefix (mkExtCall (prefix--"ext")))).
+Proof.
+  repeat autounfold with ModuleDefs.
+    unfold TraceInclusion.
+  intros.
+  exists o1, ls1.
+  repeat split; auto; intros; unfold nthProp2; intros; try destruct (nth_error ls1 i) ; auto; repeat split; intros; try firstorder.
+Qed.
+
+Theorem produce_consume_refinement (prefix: string):
+  TraceInclusion (Foo'mod (mkProduceConsume prefix (mkExtCall (prefix--"ext"))))
+                 (flattened_ModWf (module'mkProducerConsumer.wellformed_mkProducerConsumer prefix (mkExtCall (prefix--"ext")))).
+Proof.
+  repeat autounfold with ModuleDefs.
+    unfold TraceInclusion.
+  intros.
+  exists o1, ls1.
+  repeat split; auto; intros; unfold nthProp2; intros; try destruct (nth_error ls1 i) ; auto; repeat split; intros; try firstorder.
 Qed.
